Build.v
@@ -32,80 +32,75 @@ Variables blockType1 blockType2 opType1 opType2 accType : Set.
 Variable binfo : BlockInfo blockType1 blockType2 opType1 opType2.
 Variable oinfo : OpInfo maxReg accType opType1 opType2.
 
-(*
 (* For each register that is explicitly referenced by the operation, build up
    a [Interval] which excludes this register from use, but only at specific
    one-position wide ranges. *)
-Definition setIntervalsForRegs
-  `(regs : Vec (option (BoundedInterval (pos.+1).*2.+1)) maxReg)
-  (regRefs : seq PhysReg) :
-  Vec (option (BoundedInterval pos.*2.+1)) maxReg.
-Proof.
-  have regs' := regs.
-  move/(vmap (option_map (transportBoundedInterval _))) in regs'.
-  have Hleq : pos.*2.+1 <= (pos.+1).*2.+1.
-    by ordered.
-  specialize (regs' pos.*2.+1 Hleq).
-  apply: foldl _ regs' regRefs => regs' reg.
+(* Definition setIntervalsForRegs *)
+(*   `(regs : Vec (option (BoundedInterval (pos.+1).*2.+1)) maxReg) *)
+(*   (regRefs : seq PhysReg) : *)
+(*   Vec (option (BoundedInterval pos.*2.+1)) maxReg. *)
+(* Proof. *)
+(*   have regs' := regs. *)
+(*   move/(vmap (option_map (transportBoundedInterval _))) in regs'. *)
+(*   have Hleq : pos.*2.+1 <= (pos.+1).*2.+1. *)
+(*     by ordered. *)
+(*   specialize (regs' pos.*2.+1 Hleq). *)
+(*   apply: foldl _ regs' regRefs => regs' reg. *)
 
-  set upos := {| uloc   := pos.*2.+1
-               ; regReq := true |}.
-  have Hodd : odd upos by rewrite /= odd_double.
-  have H : pos.*2.+1 <= pos.*2.+1 < pos.*2.+2 by ordered.
+(*   set upos := {| uloc   := pos.*2.+1 *)
+(*                ; regReq := true |}. *)
+(*   have Hodd : odd upos by rewrite /= odd_double. *)
+(*   have H : pos.*2.+1 <= pos.*2.+1 < pos.*2.+2 by ordered. *)
 
-  pose rd := {| rbeg := uloc upos
-              ; rend := (uloc upos).+1
-              ; ups  := [:: upos] |}.
-  have r : Range rd.
-    rewrite /rd.
-    constructor=> //=.
-      by constructor; constructor.
-    by apply/andP; split.
+(*   pose rd := {| rbeg := uloc upos *)
+(*               ; rend := (uloc upos).+1 *)
+(*               ; ups  := [:: upos] |}. *)
+(*   have r : Range rd. *)
+(*     rewrite /rd. *)
+(*     constructor=> //=. *)
+(*       by constructor; constructor. *)
+(*     by apply/andP; split. *)
 
-  apply: (vreplace regs' reg _).
-  apply: Some _.
-  case: (vnth regs reg) => [[[d i] /= Hlt]|];
-    last exact: exist _ (exist _ _ (I_Sing 0 Whole r)) _.
+(*   apply: (vreplace regs' reg _). *)
+(*   apply: Some _. *)
+(*   case: (vnth regs reg) => [[[d i] /= Hlt]|]; *)
+(*     last exact: exist _ (exist _ _ (I_Sing 0 Whole r)) _. *)
 
-  case: d => [iv ib ie ik rds] in i Hlt *.
-  rewrite /= in Hlt.
-  have Hrds: rend rd < rbeg (NE_head rds).1.
-    by rewrite doubleS in Hlt.
-  move: (Interval_exact_beg i)
-        (Interval_exact_end i) => /= Hbeg Hend.
-  move: Hbeg Hend i => -> -> i.
-  rewrite /BoundedInterval.
-  by exists (exist _ _ (I_Cons (r:=packRange r) i Hrds)).
-Defined.
-*)
+(*   case: d => [iv ib ie ik rds] in i Hlt *. *)
+(*   rewrite /= in Hlt. *)
+(*   have Hrds: rend rd < rbeg (NE_head rds).1. *)
+(*     by rewrite doubleS in Hlt. *)
+(*   move: (Interval_exact_beg i) *)
+(*         (Interval_exact_end i) => /= Hbeg Hend. *)
+(*   move: Hbeg Hend i => -> -> i. *)
+(*   rewrite /BoundedInterval. *)
+(*   by exists (exist _ _ (I_Cons (r:=packRange r) i Hrds)). *)
+(* Defined. *)
 
-(*
-Definition UsePosList (pos : nat) :=
-  { us : seq (UsePos * VarKind)
-  | StronglySorted (fun x y => upos_lt (fst x) (fst y)) us
-  & if us is u :: _ then pos <= fst u else True
-  }.
+(* Definition UsePosList (pos : nat) := *)
+(*   { us : seq (UsePos * VarKind) *)
+(*   | StronglySorted (fun x y => upos_lt (fst x) (fst y)) us *)
+(*   & if us is u :: _ then pos <= fst u else True *)
+(*   }. *)
 
-Definition appendVar (pos : nat) (var : VarInfo)
-  (p : UsePosList (pos.+1).*2.+1) : UsePosList pos.*2.+1.
-Proof.
-  move: p => [us Hsort H].
-  set upos := {| uloc   := pos.*2.+1
-               ; regReq := regRequired var |}.
-  have Hodd : odd upos by rewrite /= odd_double.
-  set knd := varKind var.
-  exists ((upos, knd) :: us) => //=.
-  constructor=> //.
-  case: us => //= [u us] in Hsort H *.
-  constructor=> //.
-    by ordered.
-  inversion Hsort; subst.
-  by match_all.
-Defined.
-*)
+(* Definition appendVar (pos : nat) (var : VarInfo) *)
+(*   (p : UsePosList (pos.+1).*2.+1) : UsePosList pos.*2.+1. *)
+(* Proof. *)
+(*   move: p => [us Hsort H]. *)
+(*   set upos := {| uloc   := pos.*2.+1 *)
+(*                ; regReq := regRequired var |}. *)
+(*   have Hodd : odd upos by rewrite /= odd_double. *)
+(*   set knd := varKind var. *)
+(*   exists ((upos, knd) :: us) => //=. *)
+(*   constructor=> //. *)
+(*   case: us => //= [u us] in Hsort H *. *)
+(*   constructor=> //. *)
+(*     by ordered. *)
+(*   inversion Hsort; subst. *)
+(*   by match_all. *)
+(* Defined. *)
 
 (*
-
 block   range   first    last      range   ranges   ranges   block
 beg     beg     use pos  use pos   end     beg      end      end
 |       |       |              |       |   |             |       |
@@ -134,7 +129,6 @@ is appended to the beginning of ranges, two scenarios may occur: if "range end
 == ranges beg", then the first range in ranges simply extend to include the
 range; otherwise, the new range is prepended normally into the sorted list of
 ranges.
-
 *)
 
 Definition RangeCursor b pos mid e :=
@@ -148,7 +142,8 @@ Definition emptyRangeCursor (b pos e : nat) (H : b < pos <= e) :
   RangeCursor b pos pos e.
 Proof.
   have Hsz : b.*2.+1 < pos.*2.+1 by undoubled.
-  exists (emptyBoundedRange Hsz, emptySortedRanges) => /=.
+  exists (emptyBoundedRange Hsz (odd_double_plus _),
+          emptySortedRanges) => /=.
   by undoubled.
 Defined.
 
@@ -162,17 +157,17 @@ Proof.
   by case: (ups r.1.1) => /= [|u us] in H1 *; ordered.
 Defined.
 
-Definition RangeCursor_shiftup {b b' pos mid e}
-  (c : RangeCursor b pos mid e)
-  (Hlt : b.*2.+1 <= b'.*2.+1 <= pos.*2.+1) : RangeCursor b' pos mid e.
-Proof.
-  move: c => [[[r H] /= rs] /andP [H1 /andP [H2 H3]]] in Hlt *.
-  have Hsh: if ups r.1 is u :: _
-            then b'.*2.+1 <= u
-            else b'.*2.+1 < rend r.1 by admit.
-  pose r' := Range_shiftup r.2 Hsh.
-  by apply: exist _ (exist _ r' _, rs) _; ordered.
-Defined.
+(* Definition RangeCursor_shiftup {b b' pos mid e} *)
+(*   (c : RangeCursor b pos mid e) *)
+(*   (Hlt : b.*2.+1 <= b'.*2.+1 <= pos.*2.+1) : RangeCursor b' pos mid e. *)
+(* Proof. *)
+(*   move: c => [[[r H] /= rs] /andP [H1 /andP [H2 H3]]] in Hlt *. *)
+(*   have Hsh: if ups r.1 is u :: _ *)
+(*             then b'.*2.+1 <= u *)
+(*             else b'.*2.+1 < rend r.1 by admit. *)
+(*   pose r' := Range_shiftup r.2 Hsh. *)
+(*   by apply: exist _ (exist _ r' _, rs) _; ordered. *)
+(* Defined. *)
 
 Definition FloatingCursor b pos e :=
   { p : { n : nat | pos <= n } & RangeCursor b pos p.1 e }.
@@ -244,21 +239,21 @@ Definition varKindLtn (x y : VarKind) : bool :=
   | _, _         => true
   end.
 
-Lemma RangeCursor_pos_mid {b pos mid e} : RangeCursor b pos mid e -> pos <= mid.
-Proof.
-  move=> [[[r Hr] [rs Hsort Hlt]] /= /andP [H1 /andP [H2 H3]]].
-  move: (Range_end_bounded r.2) => /= Hbound.
-  move: (Range_sorted r.2) => /= Hsorted.
-  rewrite -leq_double.
-  apply/leq_addn1r.
-  case: (ups r.1) => /= [|u us] in H3 Hbound Hsorted *.
-    by ordered.
-  move/andP: Hr => [Hr1 Hr2].
-  apply: leq_trans _ Hr2.
-  inv Hsorted.
-  move: (Forall_last_ltn Hbound H5) => H6.
-  by ordered.
-Qed.
+(* Lemma RangeCursor_pos_mid {b pos mid e} : RangeCursor b pos mid e -> pos <= mid. *)
+(* Proof. *)
+(*   move=> [[[r Hr] [rs Hsort Hlt]] /= /andP [H1 /andP [H2 H3]]]. *)
+(*   move: (Range_end_bounded r.2) => /= Hbound. *)
+(*   move: (Range_sorted r.2) => /= Hsorted. *)
+(*   rewrite -leq_double. *)
+(*   apply/leq_addn1r. *)
+(*   case: (ups r.1) => /= [|u us] in H3 Hbound Hsorted *. *)
+(*     by ordered. *)
+(*   move/andP: Hr => [Hr1 Hr2]. *)
+(*   apply: leq_trans _ Hr2. *)
+(*   inv Hsorted. *)
+(*   move: (Forall_last_ltn Hbound H5) => H6. *)
+(*   by ordered. *)
+(* Qed. *)
 
 Definition handleVars_combine {b pos e} (H : b <= pos) (vid : nat)
   (range : FloatingCursor b pos.+1 e) (vars : bool * seq VarKind) :
@@ -287,11 +282,11 @@ Proof.
        use position into that range.  We also shift up the beginning of the
        range, since it may begin here.  By doing this iteratively for each
        variable, we determine when the range truly starts. *)
-    move: br srs => [r Hr] [rs Hsort Hlt] in H1 H3 E Hupos *.
-    pose r1 := Range_shiftup (b:=upos) r.2 Hupos.
+    move: br srs => [r Hr] [rs Hsort Hlt] /= in H1 H3 E Hupos *.
+    pose r1 := Range_shiftup (b:=upos) r.2 Hodd Hupos.
 
     have Hloc: rbeg r1.1 <= upos < head_or_end r1.1.
-      have Hsh: r1 = Range_shiftup r.2 Hupos by [].
+      have Hsh: r1 = Range_shiftup r.2 Hodd Hupos by [].
       rewrite /head_or_end /head_or.
       move: (Range_shiftup_spec Hsh) => [-> -> ->].
       clear Hsh r1.
@@ -313,40 +308,47 @@ Proof.
 
   - (* Otherwise, we must create a new [BoundedRange], and merge the previous
        one into the [SortedRanges]. *)
-    case U: ((pos.+1).*2.+1 <= rbeg br.1.1).
-      pose r1 := newRange Hodd.
-
-      have Hloc: b.*2.+1 <= (pos.+1).*2.+1 <= rbeg br.1.1.
+    case Hloc: (rbeg br.1.1 <= upos).
+    + have U: rbeg br.1.1 <= upos < head_or_end br.1.1
         by ordered.
+      pose r1 := Range_cons Hodd br.1.2 U.
+      apply: Some _.
+      apply: existT _ (exist _ mid _) _ => //=.
+        by ordered.
+      move=> _.
+      apply: exist _ (exist _ r1 _, srs) _ => /=.
+      * clear -br.
+        move: br => [? Hr].
+        exact: Hr.
+      * move=> Hr.
+        by undoubled.
+
+    + pose r1 := newRange Hodd.
+
+      move/negbT in Hloc.
+      rewrite -ltnNge /= in Hloc.
+
+      have Hspan: b.*2.+1 <= (pos.+1).*2.+1 <= rbeg br.1.1.
+        apply/andP; split=> //.
+        rewrite doubleS.
+        simpl in E.
+        move: (Range_beg_odd br.1.2) => Hbegodd.
+        apply: ltn_odd => //.
+        by apply/andP; split.
 
       apply: Some (existT _ (exist _ pos.+1 _)
                      (exist _
                         (exist _ r1 _, _) _)) => //= _.
-      + by undoubled.
-      + exact: (prependRange srs Hloc).1.
-      + move=> _.
-        case: (prependRange srs Hloc) => [p /= spec].
+      * by undoubled.
+      * exact: (prependRange srs Hspan).1.
+      * move=> _.
+        case: (prependRange srs Hspan) => [p /= spec].
         apply/andP; split=> /=;
           last by undoubled.
         rewrite -spec.
-        have Hmid': (pos.+1).*2.+1 <= mid.*2.+1 by admit.
+        have Hmid': (pos.+1).*2.+1 <= mid.*2.+1.
+          by undoubled.
         exact: (last_leq H1 Hmid').
-
-    have Hloc: rbeg br.1.1 <= upos < head_or_end br.1.1.
-      admit.
-    pose r2 := Range_cons Hodd br.1.2 Hloc.
-
-    rewrite /= in br H3 E Hupos U Hloc r2 srs H1.
-    apply: Some _.
-    apply: existT _ (exist _ mid _) _ => //=.
-      by ordered.
-    move=> _.
-    apply: exist _ (exist _ r2 _, srs) _ => /=.
-    + clear -br.
-      move: br => [? Hr].
-      exact: Hr.
-    + move=> Hr.
-      by undoubled.
 Defined.
 
 Definition handleVars_onlyRanges {b pos e}
@@ -389,6 +391,7 @@ Proof.
     + case: (Input \in kinds); by undoubled.
     + case: (Output \in kinds); by undoubled.
     + by constructor; constructor.
+    + case: (Input \in kinds); by exact: odd_double_plus.
     + by rewrite odd_double.
   - move=> r.
     case: (Input \in kinds);
@@ -448,13 +451,13 @@ Definition reduceOp {b pos e} (block : blockType1) (op : opType1)
   handleVars refs' Hlt ranges.
 
 Definition reduceBlock {pos} (block : blockType1) :
-  let sz := size (blockOps binfo block) in
+  let sz := blockSize binfo block in
   let b := pos in
   let e := pos + sz in
   PendingRanges b (pos + sz) e -> PendingRanges b pos e.
 Proof.
   move=> sz b e.
-  rewrite /sz.
+  rewrite /sz /blockSize.
   elim: (blockOps binfo block) => [|o os IHos] /=.
     by rewrite !addn0.
   rewrite !addnS.
@@ -463,185 +466,185 @@ Proof.
   exact: IHos.
 Defined.
 
-Definition computeRanges (b : nat) (block : blockType1) (liveOuts : IntSet) :
-  SSError + IntMap (seq (nat * nat) * seq UsePos) :=
-  (* for each block b in blocks in reverse order do
-       int block_from = b.first_op.id
-       int block_to = b.last_op.id + 2
+(* Definition computeRanges (b : nat) (block : blockType1) (liveOuts : IntSet) : *)
+(*   SSError + IntMap (seq (nat * nat) * seq UsePos) := *)
+(*   (* for each block b in blocks in reverse order do *)
+(*        int block_from = b.first_op.id *)
+(*        int block_to = b.last_op.id + 2 *)
 
-       for each operand opr in b.live_out do
-         intervals[opr].add_range(block_from, block_to)
-       end for
+(*        for each operand opr in b.live_out do *)
+(*          intervals[opr].add_range(block_from, block_to) *)
+(*        end for *)
 
-       for each operation op in b.operations in reverse order do
-         visitor.visit(op)
+(*        for each operation op in b.operations in reverse order do *)
+(*          visitor.visit(op) *)
 
-         if visitor.has_call then
-           for each physical register reg do
-             intervals[reg].add_range(op.id, op.id + 1)
-           end for
-         end if
+(*          if visitor.has_call then *)
+(*            for each physical register reg do *)
+(*              intervals[reg].add_range(op.id, op.id + 1) *)
+(*            end for *)
+(*          end if *)
 
-         for each virtual or physical register opr in visitor.output_oprs do
-           intervals[opr].first_range.from = op.id
-           intervals[opr].add_use_pos(op.id, use_kind_for(op, opr))
-         end for
+(*          for each virtual or physical register opr in visitor.output_oprs do *)
+(*            intervals[opr].first_range.from = op.id *)
+(*            intervals[opr].add_use_pos(op.id, use_kind_for(op, opr)) *)
+(*          end for *)
 
-         for each virtual or physical register opr in visitor.temp_oprs do
-           intervals[opr].add_range(op.id, op.id + 1)
-           intervals[opr].add_use_pos(op.id, use_kind_for(op, opr))
-         end for
+(*          for each virtual or physical register opr in visitor.temp_oprs do *)
+(*            intervals[opr].add_range(op.id, op.id + 1) *)
+(*            intervals[opr].add_use_pos(op.id, use_kind_for(op, opr)) *)
+(*          end for *)
 
-         for each virtual or physical register opr in visitor.input_oprs do
-           intervals[opr].add_range(block_from, op.id)
-           intervals[opr].add_use_pos(op.id, use_kind_for(op, opr))
-         end for
-       end for
-     end for *)
-  let endb := b + size (blockOps binfo block) in
+(*          for each virtual or physical register opr in visitor.input_oprs do *)
+(*            intervals[opr].add_range(block_from, op.id) *)
+(*            intervals[opr].add_use_pos(op.id, use_kind_for(op, opr)) *)
+(*          end for *)
+(*        end for *)
+(*      end for *) *)
+(*   let endb := b + blockSize binfo block in *)
 
-  let m := IntSet_forFold emptyIntMap liveOuts $ fun m vid =>
-    IntMap_insert (maxReg + vid) ([:: (b, endb)], [::]) m in
+(*   let m := IntSet_forFold emptyIntMap liveOuts $ fun m vid => *)
+(*     IntMap_insert (maxReg + vid) ([:: (b, endb)], [::]) m in *)
 
-  let go n op rest := if rest isn't inr m1 then rest else
-    let pos := (b + n).*2.+1 in
-    let: refs := opRefs oinfo op in
+(*   let go n op rest := if rest isn't inr m1 then rest else *)
+(*     let pos := (b + n).*2.+1 in *)
+(*     let: refs := opRefs oinfo op in *)
 
-    let recordPosRange vid m :=
-      let consRange x mxs :=
-        if mxs is Some (xs, ys)
-        then Some (x :: xs, ys)
-        else Some ([:: x], [::]) in
-      IntMap_alter (consRange (pos, pos.+1)) vid m in
+(*     let recordPosRange vid m := *)
+(*       let consRange x mxs := *)
+(*         if mxs is Some (xs, ys) *)
+(*         then Some (x :: xs, ys) *)
+(*         else Some ([:: x], [::]) in *)
+(*       IntMap_alter (consRange (pos, pos.+1)) vid m in *)
 
-    (* If this is a call operation, block every register. *)
-    let m2 :=
-      if opKind oinfo op is IsCall
-      then let fix go m n := match n with
-        | O => m
-        | S n => recordPosRange n (go m n)
-        end in
-        go m1 maxReg
-      else m1 in
+(*     (* If this is a call operation, block every register. *) *)
+(*     let m2 := *)
+(*       if opKind oinfo op is IsCall *)
+(*       then let fix go m n := match n with *)
+(*         | O => m *)
+(*         | S n => recordPosRange n (go m n) *)
+(*         end in *)
+(*         go m1 maxReg *)
+(*       else m1 in *)
 
-    let upos v := {| uloc   := pos
-                   ; regReq := regRequired v |} in
+(*     let upos v := {| uloc   := pos *)
+(*                    ; regReq := regRequired v |} in *)
 
-    (* First consider the output variables. *)
-    let outputs := [seq v <- refs | varKind v == Output] in
-    let m3 := forFold (inr m2) outputs $ fun acc v =>
-      if acc isn't inr m3 then acc else
-      match IntMap_lookup (varId v) m3 with
-      | None => inl EOutputVarMissingInput
-      | Some (nil, _) => inl EOutputVarMissingInput
-      | Some ((b, e) :: ranges, uses) =>
-        let x := ((pos, e) :: ranges, (upos v) :: uses) in
-        inr (IntMap_insert (varId v) x m3)
-      end in
-    if m3 isn't inr m3 then m3 else
+(*     (* First consider the output variables. *) *)
+(*     let outputs := [seq v <- refs | varKind v == Output] in *)
+(*     let m3 := forFold (inr m2) outputs $ fun acc v => *)
+(*       if acc isn't inr m3 then acc else *)
+(*       match IntMap_lookup (varId v) m3 with *)
+(*       | None => inl undefined (* EOutputVarMissingInput *) *)
+(*       | Some (nil, _) => inl undefined (* EOutputVarMissingInput *) *)
+(*       | Some ((b, e) :: ranges, uses) => *)
+(*         let x := ((pos, e) :: ranges, (upos v) :: uses) in *)
+(*         inr (IntMap_insert (varId v) x m3) *)
+(*       end in *)
+(*     if m3 isn't inr m3 then m3 else *)
 
-    let record vid x y m :=
-      let go x y ms :=
-        if ms is Some (xs, ys)
-        then Some (x :: xs, y :: ys)
-        else Some ([:: x], [:: y]) in
-      IntMap_alter (go x y) vid m in
+(*     let record vid x y m := *)
+(*       let go x y ms := *)
+(*         if ms is Some (xs, ys) *)
+(*         then Some (x :: xs, y :: ys) *)
+(*         else Some ([:: x], [:: y]) in *)
+(*       IntMap_alter (go x y) vid m in *)
 
-    (* Next, consider the temp variables. *)
-    let temps := [seq v <- refs | varKind v == Temp] in
-    let m4 := forFold (inr m3) temps $ fun acc v =>
-      if acc isn't inr m4 then acc else
-      inr $ record (varId v) (pos, pos.+1) (upos v) m4 in
-    if m4 isn't inr m4 then m4 else
+(*     (* Next, consider the temp variables. *) *)
+(*     let temps := [seq v <- refs | varKind v == Temp] in *)
+(*     let m4 := forFold (inr m3) temps $ fun acc v => *)
+(*       if acc isn't inr m4 then acc else *)
+(*       inr $ record (varId v) (pos, pos.+1) (upos v) m4 in *)
+(*     if m4 isn't inr m4 then m4 else *)
 
-    (* Last, consider the input variables. *)
-    let inputs := [seq v <- refs | varKind v == Input] in
-    forFold (inr m4) inputs $ fun acc v =>
-      if acc isn't inr m5 then acc else
-      inr $ record (varId v) (b, pos) (upos v) m5 in
+(*     (* Last, consider the input variables. *) *)
+(*     let inputs := [seq v <- refs | varKind v == Input] in *)
+(*     forFold (inr m4) inputs $ fun acc v => *)
+(*       if acc isn't inr m5 then acc else *)
+(*       inr $ record (varId v) (b, pos) (upos v) m5 in *)
 
-  foldr_with_index go (inr m) (blockOps binfo block).
+(*   foldr_with_index go (inr m) (blockOps binfo block). *)
 
-Program Fixpoint mergeContiguousRanges (ranges : seq (nat * nat))
-  {measure (size ranges)} : seq (nat * nat) :=
-  match ranges with
-  | (xb, xe) :: (yb, ye) :: xs =>
-    if xe == yb
-    then mergeContiguousRanges ((xb, ye) :: xs)
-    else (xb, xe) :: mergeContiguousRanges ((yb, ye) :: xs)
-  | _ => ranges
-  end.
+(* Program Fixpoint mergeContiguousRanges (ranges : seq (nat * nat)) *)
+(*   {measure (size ranges)} : seq (nat * nat) := *)
+(*   match ranges with *)
+(*   | (xb, xe) :: (yb, ye) :: xs => *)
+(*     if xe == yb *)
+(*     then mergeContiguousRanges ((xb, ye) :: xs) *)
+(*     else (xb, xe) :: mergeContiguousRanges ((yb, ye) :: xs) *)
+(*   | _ => ranges *)
+(*   end. *)
 
-Fixpoint collectUses (ranges : seq (nat * nat)) (uses : seq UsePos) :
-  seq ((nat * nat) * seq UsePos) :=
-  match ranges with
-  | [::] => [::]
-  | cons (xb, xe) xs =>
-    ((xb, xe), [seq u <- uses | xb <= uloc u < xe])
-      :: collectUses xs [seq u <- uses | ~~ (xb <= uloc u < xe)]
-  end.
+(* Fixpoint collectUses (ranges : seq (nat * nat)) (uses : seq UsePos) : *)
+(*   seq ((nat * nat) * seq UsePos) := *)
+(*   match ranges with *)
+(*   | [::] => [::] *)
+(*   | cons (xb, xe) xs => *)
+(*     ((xb, xe), [seq u <- uses | xb <= uloc u < xe]) *)
+(*       :: collectUses xs [seq u <- uses | ~~ (xb <= uloc u < xe)] *)
+(*   end. *)
 
-Definition compileRanges (ranges : seq (nat * nat)) (uses : seq UsePos) :
-  option { pos : nat & SortedRanges pos }.
-Proof.
-  case: ranges => [|[xb xe] xs].
-    exact: None.
-  pose ranges0 := (xb, xe) :: xs.
-  pose ranges1 := mergeContiguousRanges ranges0.
-  pose ranges2 := collectUses ranges1 uses.
-  apply: foldr _ (Some (existT _ xb emptySortedRanges)) ranges2.
-  move=> [[rb re] ruses].
-  case=> [[pos rest]|]; last exact: None.
-  pose rd' := {| rbeg := rb
-               ; rend := re
-               ; ups  := ruses |}.
-  have r': Range rd' by admit.
-  case E: (rend rd' < pos); last exact: None.
-  apply: Some _.
-  exists (minn pos rb).
-  move: (consRange r' rest E).
-  apply: transportSortedRanges.
-  exact: geq_minr.
-Defined.
+(* Definition compileRanges (ranges : seq (nat * nat)) (uses : seq UsePos) : *)
+(*   option { pos : nat & SortedRanges pos }. *)
+(* Proof. *)
+(*   case: ranges => [|[xb xe] xs]. *)
+(*     exact: None. *)
+(*   pose ranges0 := (xb, xe) :: xs. *)
+(*   pose ranges1 := mergeContiguousRanges ranges0. *)
+(*   pose ranges2 := collectUses ranges1 uses. *)
+(*   apply: foldr _ (Some (existT _ xb emptySortedRanges)) ranges2. *)
+(*   move=> [[rb re] ruses]. *)
+(*   case=> [[pos rest]|]; last exact: None. *)
+(*   pose rd' := {| rbeg := rb *)
+(*                ; rend := re *)
+(*                ; ups  := ruses |}. *)
+(*   have r': Range rd' by admit. *)
+(*   case E: (rend rd' < pos); last exact: None. *)
+(*   apply: Some _. *)
+(*   exists (minn pos rb). *)
+(*   move: (consRange r' rest E). *)
+(*   apply: transportSortedRanges. *)
+(*   exact: geq_minr. *)
+(* Defined. *)
 
-Definition appendBuildState `(bs : BuildState (pos + sz))
-  (m : IntMap (seq (nat * nat) * seq UsePos)) : BuildState pos.
-Proof.
-  apply: {| bsVars := IntMap_mergeWithKey _ _ _ (bsVars bs) m |}.
-  - move=> vid ranges [rawRanges rawUses].
-    (* jww (2015-02-11): All these uses of [None] here represent invariants
-       that should be true of [computeRanges], but which we are not taking the
-       time to prove right now.  They should at least be reported to the user,
-       although [IntMap_mergeWithKey] makes that impossible here. *)
+(* Definition appendBuildState `(bs : BuildState (pos + sz)) *)
+(*   (m : IntMap (seq (nat * nat) * seq UsePos)) : BuildState pos. *)
+(* Proof. *)
+(*   apply: {| bsVars := IntMap_mergeWithKey _ _ _ (bsVars bs) m |}. *)
+(*   - move=> vid ranges [rawRanges rawUses]. *)
+(*     (* jww (2015-02-11): All these uses of [None] here represent invariants *)
+(*        that should be true of [computeRanges], but which we are not taking the *)
+(*        time to prove right now.  They should at least be reported to the user, *)
+(*        although [IntMap_mergeWithKey] makes that impossible here. *) *)
 
-    (* The [raw] list is a list of ranges and of use positions, which we must
-       compile into a list of sorted ranges.  The first step is to join
-       contiguous ranges. *)
-    move: (compileRanges rawRanges rawUses) => [[b newRanges]|];
-      last exact: None.
-    case H1: (last b [seq rend r.1 | r <- newRanges.1] <= (pos + sz).*2.+1);
-      last exact: None.
-    case E: (pos.*2.+1 <= b); last exact: None.
-    apply: Some _.
-    move: (SortedRanges_cat ranges H1).
-    exact: transportSortedRanges.
+(*     (* The [raw] list is a list of ranges and of use positions, which we must *)
+(*        compile into a list of sorted ranges.  The first step is to join *)
+(*        contiguous ranges. *) *)
+(*     move: (compileRanges rawRanges rawUses) => [[b newRanges]|]; *)
+(*       last exact: None. *)
+(*     case H1: (last b [seq rend r.1 | r <- newRanges.1] <= (pos + sz).*2.+1); *)
+(*       last exact: None. *)
+(*     case E: (pos.*2.+1 <= b); last exact: None. *)
+(*     apply: Some _. *)
+(*     move: (SortedRanges_cat ranges H1). *)
+(*     exact: transportSortedRanges. *)
 
-  - apply: IntMap_map _.
-    apply: transportSortedRanges.
-    rewrite ltnS leq_double.
-    exact: leq_addr.
+(*   - apply: IntMap_map _. *)
+(*     apply: transportSortedRanges. *)
+(*     rewrite ltnS leq_double. *)
+(*     exact: leq_addr. *)
 
-  - apply: IntMap_map _.
-    (* jww (2015-02-11): See note above about these uses of
-       [emptySortedRanges], which serve the same role as using [None]
-       there. *)
-    move/(uncurry compileRanges) => [[b]|];
-      last exact: emptySortedRanges.
-    case E: (pos.*2.+1 <= b); last first.
-      move=> _.
-      exact: emptySortedRanges.
-    exact: transportSortedRanges.
-Defined.
+(*   - apply: IntMap_map _. *)
+(*     (* jww (2015-02-11): See note above about these uses of *)
+(*        [emptySortedRanges], which serve the same role as using [None] *)
+(*        there. *) *)
+(*     move/(uncurry compileRanges) => [[b]|]; *)
+(*       last exact: emptySortedRanges. *)
+(*     case E: (pos.*2.+1 <= b); last first. *)
+(*       move=> _. *)
+(*       exact: emptySortedRanges. *)
+(*     exact: transportSortedRanges. *)
+(* Defined. *)
 
 Definition compileIntervals `(bs : BuildState pos) :
   (* Return the set of fixed intervals, and the set of variable intervals,
@@ -668,7 +671,7 @@ Proof.
                then emptyIntSet
                else blockLiveOut ls.
 
-  pose sz := size (blockOps binfo b).
+  pose sz := blockSize binfo b.
   case E: (0 < sz);
     last exact: IHbs pos.
 
@@ -684,27 +687,27 @@ Proof.
                                     (bsVars (IHbs endpos)) |}.
 Defined.
 
-Definition newReduceBlocks (blocks : seq blockType1)
-  (liveSets : IntMap BlockLiveSets) {pos} : SSError + BuildState pos.
-Proof.
-  elim: blocks => [|b blocks IHbs] in pos *.
-    exact: inr newBuildState.
+(* Definition newReduceBlocks (blocks : seq blockType1) *)
+(*   (liveSets : IntMap BlockLiveSets) {pos} : SSError + BuildState pos. *)
+(* Proof. *)
+(*   elim: blocks => [|b blocks IHbs] in pos *. *)
+(*     exact: inr newBuildState. *)
 
-  have bid  := blockId binfo b.
-  have outs := if IntMap_lookup bid liveSets isn't Some ls
-               then emptyIntSet
-               else blockLiveOut ls.
+(*   have bid  := blockId binfo b. *)
+(*   have outs := if IntMap_lookup bid liveSets isn't Some ls *)
+(*                then emptyIntSet *)
+(*                else blockLiveOut ls. *)
 
-  pose sz := size (blockOps binfo b).
-  case E: (0 < sz);
-    last exact: IHbs pos.
+(*   pose sz := blockSize binfo b. *)
+(*   case E: (0 < sz); *)
+(*     last exact: IHbs pos. *)
 
-  move: (IHbs (pos + sz)) => [err|bs'].
-    exact: inl err.
-  move: (computeRanges pos b outs) => [err|res].
-    exact: inl err.
-  exact: inr (appendBuildState bs' res).
-Defined.
+(*   move: (IHbs (pos + sz)) => [err|bs']. *)
+(*     exact: inl err. *)
+(*   move: (computeRanges pos b outs) => [err|res]. *)
+(*     exact: inl err. *)
+(*   exact: inr (appendBuildState bs' res). *)
+(* Defined. *)
 
 Definition buildIntervals (blocks : seq blockType1)
   (liveSets : IntMap BlockLiveSets) : SSError + ScanStateSig maxReg InUse :=
@@ -743,10 +746,10 @@ Definition buildIntervals (blocks : seq blockType1)
     (*    end) *)
     (fun (bs : BuildState 0) =>
        let: (regs, vars) := compileIntervals bs in
-       let s1   := ScanState_setFixedIntervals s0 regs in
-       let s2   := packScanState s1 in
-       let s3   := IntMap_foldlWithKey (handleVar 0) s2 (bsVars bs) in
-       let s4   := ScanState_finalize s3.2 in
+       let s1 := ScanState_setFixedIntervals s0 regs in
+       let s2 := packScanState s1 in
+       let s3 := IntMap_foldlWithKey (handleVar 0) s2 (bsVars bs) in
+       let s4 := ScanState_finalize s3.2 in
        inr $ packScanState s4)
     (reduceBlocks bs liveSets).
 
