NonEmpty.v
@@ -58,13 +58,13 @@ Fixpoint NE_map {a b : Type} (f : a -> b) (ne : NonEmpty a) : NonEmpty b :=
     | NE_Cons x xs => NE_Cons (f x) (NE_map f xs)
   end.
 
-Lemma NE_map_head : forall a b (f : a -> b) xs,
-  NE_head (NE_map f xs) = f (NE_head xs).
-Proof. by move=> a b f; elim=> [x|x xs IHxs] //=. Qed.
+(* Lemma NE_map_head : forall a b (f : a -> b) xs, *)
+(*   NE_head (NE_map f xs) = f (NE_head xs). *)
+(* Proof. by move=> a b f; elim=> [x|x xs IHxs] //=. Qed. *)
 
-Lemma NE_map_last : forall a b (f : a -> b) xs,
-  NE_last (NE_map f xs) = f (NE_last xs).
-Proof. by move=> a b f; elim=> [x|x xs IHxs] //=. Qed.
+(* Lemma NE_map_last : forall a b (f : a -> b) xs, *)
+(*   NE_last (NE_map f xs) = f (NE_last xs). *)
+(* Proof. by move=> a b f; elim=> [x|x xs IHxs] //=. Qed. *)
 
 Definition NE_foldl {a b : Type} (f : a -> b -> a) (z : a) (ne : NonEmpty b) : a :=
   foldl f z ne.
@@ -114,13 +114,13 @@ Lemma NE_Forall_head : forall P (xs : NonEmpty A),
   NE_Forall P xs -> P (NE_head xs).
 Proof. induction xs; intros; inversion H0; assumption. Qed.
 
-Lemma NE_Forall_last : forall P (xs : NonEmpty A),
-  NE_Forall P xs -> P (NE_last xs).
-Proof.
-  intros. induction xs; simpl in *.
-    inversion H0. assumption.
-  apply IHxs. inversion H0. assumption.
-Qed.
+(* Lemma NE_Forall_last : forall P (xs : NonEmpty A), *)
+(*   NE_Forall P xs -> P (NE_last xs). *)
+(* Proof. *)
+(*   intros. induction xs; simpl in *. *)
+(*     inversion H0. assumption. *)
+(*   apply IHxs. inversion H0. assumption. *)
+(* Qed. *)
 
 Lemma NE_Forall_append : forall (P : A -> Prop) xs ys,
    NE_Forall P xs /\ NE_Forall P ys <-> NE_Forall P (NE_append xs ys).
@@ -134,19 +134,19 @@ Proof.
   intuition.
 Qed.
 
-Lemma NE_Forall_impl : forall (P Q : A -> Prop), (forall a, P a -> Q a) ->
-  forall l, NE_Forall P l -> NE_Forall Q l.
-Proof.
-  intros P Q Himp l H1.
-  induction H1; firstorder.
-Qed.
+(* Lemma NE_Forall_impl : forall (P Q : A -> Prop), (forall a, P a -> Q a) -> *)
+(*   forall l, NE_Forall P l -> NE_Forall Q l. *)
+(* Proof. *)
+(*   intros P Q Himp l H1. *)
+(*   induction H1; firstorder. *)
+(* Qed. *)
 
-Lemma NE_Forall_inv : forall (P : A -> Prop) x l,
-  NE_Forall P (NE_Cons x l) -> P x /\ NE_Forall P l.
-Proof.
-  move=> P x l Hall.
-  by inversion Hall.
-Qed.
+(* Lemma NE_Forall_inv : forall (P : A -> Prop) x l, *)
+(*   NE_Forall P (NE_Cons x l) -> P x /\ NE_Forall P l. *)
+(* Proof. *)
+(*   move=> P x l Hall. *)
+(*   by inversion Hall. *)
+(* Qed. *)
 
 Section Membership.
 
@@ -175,37 +175,37 @@ Inductive NE_StronglySorted : NonEmpty A -> Prop :=
   | NE_SSorted_cons a l : NE_StronglySorted l -> NE_Forall (R a) l
                             -> NE_StronglySorted (NE_Cons a l).
 
-Lemma NE_StronglySorted_inv : forall a l,
-  NE_StronglySorted (NE_Cons a l)
-    -> NE_StronglySorted l /\ NE_Forall (R a) l.
-Proof. intros; inversion H0; auto. Qed.
+(* Lemma NE_StronglySorted_inv : forall a l, *)
+(*   NE_StronglySorted (NE_Cons a l) *)
+(*     -> NE_StronglySorted l /\ NE_Forall (R a) l. *)
+(* Proof. intros; inversion H0; auto. Qed. *)
 
-Lemma NE_StronglySorted_inv_app : forall (l1 l2 : NonEmpty A),
-  NE_StronglySorted (NE_append l1 l2)
-    -> NE_StronglySorted l1 /\ NE_StronglySorted l2.
-Proof.
-  induction l1; intros; simpl; inversion H0.
-    split; [ constructor | assumption ].
-  specialize (IHl1 l2 H3).
-  inversion IHl1.
-  split.
-    constructor. assumption.
-    apply NE_Forall_append in H4. intuition.
-  assumption.
-Qed.
+(* Lemma NE_StronglySorted_inv_app : forall (l1 l2 : NonEmpty A), *)
+(*   NE_StronglySorted (NE_append l1 l2) *)
+(*     -> NE_StronglySorted l1 /\ NE_StronglySorted l2. *)
+(* Proof. *)
+(*   induction l1; intros; simpl; inversion H0. *)
+(*     split; [ constructor | assumption ]. *)
+(*   specialize (IHl1 l2 H3). *)
+(*   inversion IHl1. *)
+(*   split. *)
+(*     constructor. assumption. *)
+(*     apply NE_Forall_append in H4. intuition. *)
+(*   assumption. *)
+(* Qed. *)
 
-Lemma NE_StronglySorted_impl_app : forall (l1 l2 : NonEmpty A),
-  NE_StronglySorted (NE_append l1 l2) -> R (NE_last l1) (NE_head l2).
-Proof.
-  intros.
-  induction l1; simpl in *.
-    inversion H0; subst.
-    apply NE_Forall_head in H4.
-    assumption.
-  apply IHl1.
-  inversion H0.
-  assumption.
-Qed.
+(* Lemma NE_StronglySorted_impl_app : forall (l1 l2 : NonEmpty A), *)
+(*   NE_StronglySorted (NE_append l1 l2) -> R (NE_last l1) (NE_head l2). *)
+(* Proof. *)
+(*   intros. *)
+(*   induction l1; simpl in *. *)
+(*     inversion H0; subst. *)
+(*     apply NE_Forall_head in H4. *)
+(*     assumption. *)
+(*   apply IHl1. *)
+(*   inversion H0. *)
+(*   assumption. *)
+(* Qed. *)
 
 End Sorted.
 
